Heap/AddEdge.v
@@ -1,0 +1,45 @@
+Require Import Coq.Lists.List.
+Require Import Coq.ZArith.ZArith.
+Require Import Coq.Classes.RelationClasses.
+Require Import PL.Monad.
+Require Import PL.Monad2.
+Require Import SetsClass.
+Require Import HEAP.Defs.
+Import SetsNotation
+       StateRelMonad
+       StateRelMonadOp
+       StateRelMonadHoare
+       MonadNotation
+       Monad.
+Local Open Scope sets.
+Local Open Scope Z.
+Local Open Scope monad.
+
+Fact add_go_left_edge_fact1: forall (v lc: Z) (V: Z -> Prop),
+  Hoare (fun s => Abs s.(heap) V)
+        (add_go_left_edge v lc)
+        (fun _ s => Abs s.(heap) V).
+Admitted.
+
+Fact add_go_left_edge_fact2: forall (v lc: Z),
+  Hoare (fun s => BinaryTree.legal s.(heap) /\ 
+                  ~ (exists x, BinaryTree.step_l s.(heap) v x) /\ 
+                  ~ (exists x, BinaryTree.step_u s.(heap) lc x))
+        (add_go_left_edge v lc)
+        (fun _ s => BinaryTree.legal s.(heap)).
+Admitted.
+
+Fact add_go_right_edge_fact1: forall (v rc: Z) (V: Z -> Prop),
+  Hoare (fun s => Abs s.(heap) V)
+        (add_go_right_edge v rc)
+        (fun _ s => Abs s.(heap) V).
+Admitted.
+
+Fact add_go_right_edge_fact2: forall (v rc: Z),
+  Hoare (fun s => BinaryTree.legal s.(heap) /\ 
+                  ~ (exists x, BinaryTree.step_r s.(heap) v x) /\ 
+                  ~ (exists x, BinaryTree.step_u s.(heap) rc x))
+        (add_go_right_edge v rc)
+        (fun _ s => BinaryTree.legal s.(heap)).
+Admitted.
+
